add support for recursive types and their corresponding compatibility lemmas

theories/logic/sem_types.v
@@ -8,6 +8,7 @@
 From iris.proofmode Require Import base tactics.
 From iris.algebra Require Import ofe.
 From iris.base_logic.lib Require Import iprop invariants.
+From iris.base_logic Require Import upred.
 
 (* Hazel Reasoning *)
 From program_logic Require Import weakest_precondition 
@@ -52,20 +53,23 @@ Definition sem_ty_ref `{!heapGS Σ} (τ : sem_ty Σ): sem_ty Σ :=
 Definition sem_ty_prod {Σ} (τ κ : sem_ty Σ) : sem_ty Σ := 
   (λ v, ∃ v₁ v₂, ⌜v = (v₁, v₂)%V⌝ ∗ τ v₁ ∗ κ v₂)%I.
 
+(* Sum type. *)
+Definition sem_ty_sum {Σ} (τ κ : sem_ty Σ) : sem_ty Σ := 
+  (λ v, ∃ v', (⌜v = InjLV v'%V⌝ ∗ τ v') ∨ (⌜ v = InjRV v'⌝ ∗ κ v'))%I.
+
 (* Linear Arrow type. *)
-Definition sem_ty_larr `{irisGS eff_lang Σ} 
-  (τ : sem_ty Σ)
+Definition sem_ty_larr `{!heapGS Σ} 
   (ρ : sem_row Σ)
+  (τ : sem_ty Σ)
   (κ : sem_ty Σ) : sem_ty Σ :=
   (λ (v : val), ∀ (w : val), τ w -∗ EWP (v w) <| ρ |> {{ κ }})%I.
 
 (* Unrestricted Arrow type. *)
 Definition sem_ty_uarr `{irisGS eff_lang Σ} 
-  (τ : sem_ty Σ)
   (ρ : sem_row Σ)
+  (τ : sem_ty Σ)
   (κ : sem_ty Σ) : sem_ty Σ :=
   (λ (v : val), ∀ (w : val), □ (τ w -∗ EWP (v w) <| ρ |> {{ κ }}))%I.
-
 
 (* Polymorphic type. *)
 Definition sem_ty_forall `{irisGS eff_lang Σ} 
@@ -85,23 +89,63 @@ Proof. solve_contractive. Qed.
 Definition sem_ty_rec {Σ} (C : sem_ty Σ → sem_ty Σ) : sem_ty Σ :=
   fixpoint (sem_ty_rec_pre C).
 
+Lemma sem_ty_equiv {Σ} v (τ τ' : sem_ty Σ) : 
+  τ ≡ τ' → τ v ≡ τ' v.
+Proof.
+  intros Hτ. unfold equiv, ofe_equiv in Hτ. 
+  simpl in Hτ. unfold discrete_fun_equiv in Hτ.
+  by apply Hτ.
+Qed.
+
+Lemma sem_ty_dist {Σ} v (τ τ' : sem_ty Σ) n : 
+  dist n τ τ' → dist n (τ v) (τ' v).
+Proof.
+  intros Hττ'. unfold dist, ofe_dist in Hττ'.
+  simpl in Hττ'. unfold discrete_fun_dist in Hττ'.
+  by apply Hττ'.
+Qed.
+
 Lemma sem_ty_rec_unfold {Σ} (C : sem_ty Σ → sem_ty Σ) `{!NonExpansive C} v :
   (sem_ty_rec C)%T v ⊣⊢ ▷ C (sem_ty_rec C)%T v.
 Proof.
-  rewrite {1}/sem_ty_rec. 
-  Fail rewrite (fixpoint_unfold (sem_ty_rec_pre C)). 
-Admitted.
+  rewrite {1}/sem_ty_rec.
+  (*          
+  ∙ f := sem_ty_rec_pre C : sem_ty → sem_ty
+  ∙ fixpoint (sem_ty_rec_pre C) : sem_ty
 
-Fixpoint is_of_list_type {Σ} (l : val) (τ : sem_ty Σ ) (xs : list val) : (iProp Σ) :=
-  match xs with
-    | [] => ⌜ l = NILV ⌝
-    | x :: xxs => ∃ tl, ⌜ l = CONSV x tl ⌝ ∗ τ x ∗ is_of_list_type tl τ xxs
-  end
-.
+  The equivalence we have from fixpoint_unfold is: 
+    fixpoint f ≡ f (fixpoint f)
 
-(* List type. *)
-Definition sem_ty_list {Σ} (τ : sem_ty Σ) : sem_ty Σ := 
-  (λ v, ∃ xs, is_of_list_type v τ xs)%I.
+    Since fixpoint f : val -d> iProp, and
+          f (fixpoint f) : val -d> iProp
+
+  We want to get that given two sem_types are equivalent,
+  if we apply them with the same value we get that 
+  the result is also equivalent.
+
+  So we want this equivalence:
+    ∀ v, fixpoint f v ≡ f (fixpoint f) v
+
+  But even though the equivalence instance for val -d> iProp
+  is just that, Coq has trouble rewriting directly with fixpoint_unfold,
+  because it is a function.
+  As a result we fistly apply sem_ty_equiv lemma *)
+  assert (fixpoint (sem_ty_rec_pre C) v ≡ sem_ty_rec_pre C (fixpoint (sem_ty_rec_pre C)) v).
+  { apply sem_ty_equiv. apply fixpoint_unfold. }
+  rewrite H. iSplit.
+  - iIntros "(%rec' & #Hrec & HC) !>".
+    set Ψ := λ τ, C τ v.
+    assert (Ψ rec' = C rec' v) by done.
+    assert (Ψ (sem_ty_rec C) = C (sem_ty_rec C) v) by done.
+    rewrite <- H0. rewrite <- H1.
+    iApply (internal_eq_rewrite rec' (sem_ty_rec C)).
+    + intros n τ τ' Hττ'. unfold Ψ. apply sem_ty_dist. 
+      by apply NonExpansive0.
+    + by iApply internal_eq_sym.
+    + iApply "HC".
+  - iIntros "HC //=". iNext. iExists (sem_ty_rec C).
+    by iFrame. 
+Qed.
 
 (* Empty Effect Row. *)
 Definition sem_row_bot {Σ} : sem_row Σ := iEff_bottom.
@@ -127,6 +171,7 @@ Notation "'𝔹'" := (sem_ty_bool) : sem_ty_scope.
 Notation "'ℤ'" := (sem_ty_int) : sem_ty_scope.
 Notation "τ '×' κ" := (sem_ty_prod τ%T κ%T)
   (at level 120, κ at level 200) : sem_ty_scope.
+Infix "+" := (sem_ty_sum) : sem_ty_scope.
 
 Notation "'Ref' τ" := (sem_ty_ref τ%T) 
   (at level 50) : sem_ty_scope.
@@ -137,19 +182,114 @@ Notation "'∀:' A , ρ , C " := (sem_ty_forall ρ (λ A, C%T))
 Notation "'∃:' A , C " := (sem_ty_exists (λ A, C%T)) 
   (at level 180) : sem_ty_scope.
 
-Notation "'List' τ" := (sem_ty_list τ%T) 
-  (at level 50) : sem_ty_scope.
+Notation "'μ:' A , C " := (sem_ty_rec (λ A, C%T)) 
+  (at level 180) : sem_ty_scope.
 
 Notation "⟨⟩" := sem_row_bot : sem_row_scope.
 Notation "τ ⇒ κ" := (sem_row_eff τ%T κ%T) 
   (at level 100, κ at level 200) : sem_row_scope.
 
-Notation "τ '-{' ρ '}-∘' κ" := (sem_ty_larr τ%T ρ%R κ%T)
+Notation "τ '-{' ρ '}-∘' κ" := (sem_ty_larr ρ%R τ%T κ%T)
   (at level 100, ρ, κ at level 200) : sem_ty_scope.
-Notation "τ ⊸ κ" := (sem_ty_larr τ%T sem_row_bot κ%T)
+Notation "τ ⊸ κ" := (sem_ty_larr sem_row_bot τ%T κ%T)
   (at level 99, κ at level 200) : sem_ty_scope.
 
-Notation "τ '-{' ρ '}->' κ" := (sem_ty_uarr τ%T ρ%R κ%T)
+Notation "τ '-{' ρ '}->' κ" := (sem_ty_uarr ρ%R τ%T κ%T)
   (at level 100, ρ, κ at level 200) : sem_ty_scope.
-Notation "τ → κ" := (sem_ty_uarr τ%T sem_row_bot κ%T)
+Notation "τ → κ" := (sem_ty_uarr sem_row_bot τ%T κ%T)
   (at level 99, κ at level 200) : sem_ty_scope.
+
+
+(* Derived Types *)
+
+Definition ListF {Σ} (τ : sem_ty Σ) := λ α, (() + (τ × α))%T.
+
+(* List type. *)
+Definition sem_ty_list {Σ} (τ : sem_ty Σ) : sem_ty Σ := 
+    sem_ty_rec (ListF τ).
+
+Notation "'List' τ" := (sem_ty_list τ%T) 
+  (at level 50) : sem_ty_scope.
+
+
+(**  Prove that type formers are non-expansive and respect setoid equality. *)
+Section types_properties.
+  Context `{!heapGS Σ}.
+
+  Ltac solve_non_expansive2 :=
+    intros m x y Hxy x' y' Hxy'; try intros ?;
+    unfold sem_ty_unit, sem_ty_int, sem_ty_bool,
+           sem_ty_prod, sem_ty_sum, sem_ty_larr,
+           sem_ty_uarr, sem_ty_ref, sem_ty_rec,
+           sem_ty_list, sem_ty_forall, sem_ty_exists;
+    repeat f_equiv; done || by apply sem_ty_dist.
+
+  Global Instance sem_ty_prod_ne : NonExpansive2 (@sem_ty_prod Σ).
+  Proof. solve_non_expansive2. Qed.
+
+  Global Instance sem_ty_sum_ne : NonExpansive2 (@sem_ty_sum Σ).
+  Proof. solve_non_expansive2. Qed.
+
+  Global Instance sem_ty_larr_ne ρ : NonExpansive2 (sem_ty_larr ρ).
+  Proof. solve_non_expansive2. Qed.
+
+  Global Instance sem_ty_uarr_ne ρ : NonExpansive2 (sem_ty_uarr ρ).
+  Proof. solve_non_expansive2. Qed.
+
+  Global Instance sem_ty_ref_ne : NonExpansive2 (@sem_ty_ref Σ _).
+  Proof. solve_non_expansive2. Qed.
+
+  Global Instance sem_ty_forall_ne n ρ :
+    Proper (pointwise_relation _ (dist n) ==> dist n) (sem_ty_forall ρ).
+  Proof. intros ????. unfold sem_ty_forall; repeat f_equiv. Qed.
+
+  Global Instance sem_ty_exist_ne n :
+    Proper (pointwise_relation _ (dist n) ==> dist n) sem_ty_exists.
+  Proof. intros ????. unfold sem_ty_exists; repeat f_equiv. 
+         unfold pointwise_relation in H. by apply sem_ty_dist. Qed.
+
+  Global Instance sem_ty_rec_ne n :
+    Proper (pointwise_relation _ (dist n) ==> dist n) (@sem_ty_rec Σ).
+  Proof.
+    intros C1 C2 HA. unfold sem_ty_rec. apply fixpoint_ne.
+    intros ??. unfold sem_ty_rec_pre. do 4 f_equiv. 
+    by apply sem_ty_dist.
+  Qed.
+
+  Global Instance sem_ty_listF_ne τ : NonExpansive (@ListF Σ τ).
+  Proof. intros ????. unfold ListF; by repeat f_equiv. Qed.
+
+  Global Instance sem_ty_prod_proper : Proper ((≡) ==> (≡) ==> (≡)) (@sem_ty_prod Σ).
+  Proof. solve_non_expansive2. Qed.
+
+  Global Instance sem_ty_sum_proper : Proper ((≡) ==> (≡) ==> (≡)) (@sem_ty_sum Σ).
+  Proof. solve_non_expansive2. Qed.
+
+  Global Instance sem_ty_larr_proper ρ : Proper ((≡) ==> (≡) ==> (≡)) (sem_ty_larr ρ).
+  Proof. solve_non_expansive2. Qed.
+
+  Global Instance sem_ty_uarr_proper ρ : Proper ((≡) ==> (≡) ==> (≡)) (sem_ty_uarr ρ).
+  Proof. solve_non_expansive2. Qed.
+
+  Global Instance sem_ty_ref_proper : Proper ((≡) ==> (≡)) (@sem_ty_ref Σ _).
+  Proof. intros ????. unfold sem_ty_ref; by repeat f_equiv. Qed.
+
+  Global Instance sem_ty_forall_proper ρ:
+    Proper (pointwise_relation _ (≡) ==> (≡)) (sem_ty_forall ρ).
+  Proof. intros ????; unfold sem_ty_forall; repeat f_equiv. Qed.
+
+  Global Instance sem_ty_exist_proper :
+    Proper (pointwise_relation _ (≡) ==>(≡)) sem_ty_exists.
+  Proof. 
+    intros ????. unfold sem_ty_exists; repeat f_equiv.
+    by apply sem_ty_equiv.
+  Qed.
+
+  Global Instance sem_ty_rec_proper :
+    Proper (pointwise_relation _ (≡) ==>(≡)) (@sem_ty_rec Σ).
+  Proof.
+    intros C1 C2 HA. apply equiv_dist=> n.
+    apply sem_ty_rec_ne=> A. by apply equiv_dist.
+  Qed.
+
+End types_properties.
